extraction/Extraction.v
@@ -27,55 +27,56 @@ Definition lgDataBytes := idxBits + tagBits + lgNumDatas.
 Definition fifoSize := 2.
 Definition idK := Bit 1.
 
-(* Temporary; just for experiment *)
-Definition pdecAN := pdecAN fifoSize rv32iDecode rv32iExecState rv32iExecNextPc
-                            rv32iOpLOAD rv32iOpSTORE rv32iOpTOHOST lgNumChildren.
+(* TODO: recover *)
 
-Definition pdecN := pdecN idxBits tagBits lgNumDatas
-                          rv32iDecode rv32iExecState rv32iExecNextPc
-                          rv32iOpLOAD rv32iOpSTORE rv32iOpTOHOST lgNumChildren.
-Definition pmFifos := pmFifos fifoSize idxBits tagBits lgNumDatas lgDataBytes lgNumChildren.
+(* Definition pdecAN := pdecAN fifoSize rv32iDecode rv32iExecState rv32iExecNextPc *)
+(*                             rv32iOpLOAD rv32iOpSTORE rv32iOpTOHOST lgNumChildren. *)
 
-Definition l1Con := ((modFromMeta (l1Cache idxBits tagBits lgNumDatas lgDataBytes
-                                           idK lgNumChildren))
-                       ++ ((modFromMeta (l1cs idxBits lgNumChildren))
-                             ++ (modFromMeta (l1tag idxBits tagBits lgNumChildren))
-                             ++ (modFromMeta (l1line idxBits lgNumDatas lgDataBytes lgNumChildren)))
-                       ++ ((modFromMeta (fifoRqToP idxBits tagBits idK fifoSize lgNumChildren))
-                             ++ (modFromMeta (fifoRsToP idxBits tagBits lgNumDatas lgDataBytes
-                                                        fifoSize lgNumChildren))
-                             ++ (modFromMeta (fifoFromP idxBits tagBits lgNumDatas lgDataBytes
-                                                        idK fifoSize lgNumChildren))))%kami.
+(* Definition pdecN := pdecN idxBits tagBits lgNumDatas *)
+(*                           rv32iDecode rv32iExecState rv32iExecNextPc *)
+(*                           rv32iOpLOAD rv32iOpSTORE rv32iOpTOHOST lgNumChildren. *)
+(* Definition pmFifos := pmFifos fifoSize idxBits tagBits lgNumDatas lgDataBytes lgNumChildren. *)
 
-Definition memDirCCon := ((modFromMeta (memDir idxBits tagBits lgNumDatas lgDataBytes
-                                               idK lgNumChildren))
-                            ++ (modFromMeta (mline idxBits tagBits lgNumDatas lgDataBytes))
-                            ++ (modFromMeta (mdir idxBits tagBits lgNumChildren)))%kami.
+(* Definition l1Con := ((modFromMeta (l1Cache idxBits tagBits lgNumDatas lgDataBytes *)
+(*                                            idK lgNumChildren)) *)
+(*                        ++ ((modFromMeta (l1cs idxBits lgNumChildren)) *)
+(*                              ++ (modFromMeta (l1tag idxBits tagBits lgNumChildren)) *)
+(*                              ++ (modFromMeta (l1line idxBits lgNumDatas lgDataBytes lgNumChildren))) *)
+(*                        ++ ((modFromMeta (fifoRqToP idxBits tagBits idK fifoSize lgNumChildren)) *)
+(*                              ++ (modFromMeta (fifoRsToP idxBits tagBits lgNumDatas lgDataBytes *)
+(*                                                         fifoSize lgNumChildren)) *)
+(*                              ++ (modFromMeta (fifoFromP idxBits tagBits lgNumDatas lgDataBytes *)
+(*                                                         idK fifoSize lgNumChildren))))%kami. *)
 
-Definition childParentCCon := ((modFromMeta (childParent idxBits tagBits lgNumDatas lgDataBytes
-                                                         idK lgNumChildren))
-                                 ++ (modFromMeta (fifoRqFromC idxBits tagBits
-                                                              idK fifoSize lgNumChildren))
-                                 ++ (modFromMeta (fifoRsFromC idxBits tagBits lgNumDatas lgDataBytes
-                                                              fifoSize lgNumChildren))
-                                 ++ (modFromMeta (fifoToC idxBits tagBits lgNumDatas lgDataBytes
-                                                          idK fifoSize lgNumChildren)))%kami.
+(* Definition memDirCCon := ((modFromMeta (memDir idxBits tagBits lgNumDatas lgDataBytes *)
+(*                                                idK lgNumChildren)) *)
+(*                             ++ (modFromMeta (mline idxBits tagBits lgNumDatas lgDataBytes)) *)
+(*                             ++ (modFromMeta (mdir idxBits tagBits lgNumChildren)))%kami. *)
 
-Definition memCache := (l1Con ++ childParentCCon ++ memDirCCon)%kami.
+(* Definition childParentCCon := ((modFromMeta (childParent idxBits tagBits lgNumDatas lgDataBytes *)
+(*                                                          idK lgNumChildren)) *)
+(*                                  ++ (modFromMeta (fifoRqFromC idxBits tagBits *)
+(*                                                               idK fifoSize lgNumChildren)) *)
+(*                                  ++ (modFromMeta (fifoRsFromC idxBits tagBits lgNumDatas lgDataBytes *)
+(*                                                               fifoSize lgNumChildren)) *)
+(*                                  ++ (modFromMeta (fifoToC idxBits tagBits lgNumDatas lgDataBytes *)
+(*                                                           idK fifoSize lgNumChildren)))%kami. *)
 
-Definition procMemCache := (pdecN ++ pmFifos ++ memCache)%kami.
+(* Definition memCache := (l1Con ++ childParentCCon ++ memDirCCon)%kami. *)
 
-(** MODIFY targetPgm to your target program *)
-Definition targetPgm := pgmFibonacci 10.
+(* Definition procMemCache := (pdecN ++ pmFifos ++ memCache)%kami. *)
 
-(** MODIFY targetM to your target module *)
-Definition targetProcM := pdecAN.
+(* (** MODIFY targetPgm to your target program *) *)
+(* Definition targetPgm := pgmFibonacci 10. *)
 
-(** DON'T REMOVE OR MODIFY BELOW LINES *)
-Definition targetProcS := getModuleS targetProcM.
-Definition targetProcB := ModulesSToBModules targetProcS.
+(* (** MODIFY targetM to your target module *) *)
+(* Definition targetProcM := pdecAN. *)
 
-Definition target := (targetPgm, targetProcB).
+(* (** DON'T REMOVE OR MODIFY BELOW LINES *) *)
+(* Definition targetProcS := getModuleS targetProcM. *)
+(* Definition targetProcB := ModulesSToBModules targetProcS. *)
+
+(* Definition target := (targetPgm, targetProcB). *)
 
 (* Extraction "./Ocaml/Target.ml" target. *)
 
